use subtype/eqtype instead of mono/proper

theories/util/basic.v
@@ -18,3 +18,5 @@ Infix "⊛" := s_comb (left associativity, at level 50).
 Lemma surjective_pairing_fun {A B C} (f: A → B * C) :
   f = (pair ∘ (fst ∘ f) ⊛ (snd ∘ f)).
 Proof. extensionality x. by rewrite /s_comb /compose -surjective_pairing. Qed.
+
+Definition pairmap {A B A' B'} (f: A → A') (g: B → B') xy := (f xy.1, g xy.2).
